Progress with subsorts
First I tried a version of the carrier that mirrors the subsort
relation, but it didn't seem to be very helpful and didn't solve the
problem of not being able to do inversion on Prop.

So I decided to see what would happen if we used a computable relation
(crelation) for subsorting, which did allow me to do inversion and
define the model. For this, I used the original carrier as that seems
easier to generate automatically.

I tried some axioms, and one was provable but the others are really
ugly. I'm not sure I even defined them correctly (see ? comments) but I
suspect they won't simplify because of the ltac definition. However, due
to the excessive use of dependent destructions/inductions I'm not sure
if a gallina definition would look much better.

I also tried an EqDecision definition, should be possible, but
transports don't make it easy, and I didn't want to spend more time on
it. Only needed for list inclusion.

kore/src/theories/TrialSubsorts.v
@@ -75,31 +75,36 @@ Module T.
   | SymIsList
   | SymNil
   | SymCons
-  | SymInList.
+  | SymInList
+  | SymAppend.
 
   (* We prove decidable equality and finiteness of the type above. *)
   Instance DemoSyms_eq_dec : EqDecision DemoSyms.
   Proof. solve_decision. Defined.
   Program Instance DemoSyms_finite : finite.Finite DemoSyms := {
     enum := [SymZero;SymSucc;SymAdd;SymTrue;
-    SymFalse;SymIsList;SymNil;SymCons;SymInList];
+    SymFalse;SymIsList;SymNil;SymCons;SymInList;SymAppend];
   }.
   Next Obligation. compute_done. Defined.
   Final Obligation. destruct x; set_solver. Defined.
 
-  Inductive Demo_subsort : DemoSorts -> DemoSorts -> Prop :=
+  Inductive Demo_subsort : CRelationClasses.crelation DemoSorts :=
   | subsorts_refl s : Demo_subsort s s
   | kitem_is_top s : s ≠ SortK -> Demo_subsort s SortKItem.
 
-  Instance Demo_subsort_PartialOrder : PartialOrder Demo_subsort.
+  Instance Demo_subsort_PreOrder : CRelationClasses.PreOrder Demo_subsort.
   Proof.
-    apply Build_PartialOrder.
-    apply Build_PreOrder.
-    * intro s. constructor.
-    * intros s1 s2 s3 H H0.
-      invt H; invt H0; try by constructor.
-    * intros s1 s2 H H0.
-      invt H; invt H0; reflexivity.
+    split.
+    cbv. intro. left.
+    cbv. intros. inversion H; subst. assumption.
+    inversion H0; subst. assumption. assumption.
+  Defined.
+
+  Instance Demo_subsort_PartialOrder : CRelationClasses.PartialOrder eq Demo_subsort.
+  Proof.
+    cbv. intros. split; intros. rewrite H. repeat constructor.
+    destruct H. inversion d; subst. reflexivity.
+    inversion d0; subst; reflexivity.
   Defined.
 
   (* In the signature, we need to define the sorts, the variable types,
@@ -123,11 +128,12 @@ Module T.
                  | SymNil => []
                  | SymCons => [SortKItem; SortList]
                  | SymInList => [SortKItem; SortList]
+                 | SymAppend => [SortList; SortList]
                  end;
       ret_sort := fun σ => match σ with
                            | SymZero | SymSucc | SymAdd => SortNat
                            | SymTrue | SymFalse => SortBool
-                           | SymNil | SymCons => SortList
+                           | SymNil | SymCons | SymAppend => SortList
                            | SymInList | SymIsList => SortBool
                            end;
     |};
@@ -138,64 +144,160 @@ Module T.
   | c_bool (b : bool) : carrier SortBool
   | c_nil : carrier SortList
   | c_cons : carrier SortKItem -> carrier SortList -> carrier SortList
-  | c_subsort (s1 s2 : DemoSorts) (P : subsort s1 s2) (x : carrier s1) : carrier s2.
+  | c_subsort (s1 s2 : DemoSorts) (P : subsort s1 s2) (x : carrier s1) : carrier s2
+  (* This should match the subsort relation *)
+  (* | c_kitem {A} : A ≠ SortK -> carrier A -> carrier SortKItem *)
+  | c_dotk : carrier SortK.
 
-  Check c_nat 1.
-  Check c_nil.
-  Check c_cons (c_subsort _ _ _ (c_nat 1)) c_nil.
-(*   Check c_cons (c_nat 1) (c_cons (c_bool false) c_nil).
-  Check c_cons (c_nat 1) (c_cons (c_bool false) (c_cons (c_cons (c_nat 1) c_nil) c_nil)). *)
+  (* Check c_nat 1. *)
+  (* Check c_nil. *)
+  (* Check c_cons (c_kitem (eq_ind SortNat (λ x, if x is SortNat then True else False) I _) (c_nat 1)) c_nil. *)
+  (* Check c_cons (c_nat 1) (c_cons (c_bool false) c_nil). *)
+  (* Check c_cons (c_nat 1) (c_cons (c_bool false) (c_cons (c_cons (c_nat 1) c_nil) c_nil)). *)
 
+  Lemma neqs_eq {A} {a b : A} (p q : a ≠ b) : p = q.
+  Proof.
+    apply functional_extensionality. intros. destruct (p x).
+  Defined.
 
-  Program Definition DemoModel : @Model DemoSignature :=
-    mkModel_singleton
-      carrier
-      (DemoSyms_rect _
-        (c_nat 0)
-        _
-        _
-        _
-        _
-        _
-        _
-        _
-        _
-      )
-      _
-      _.
-  Next Obligation.
-    simpl.
-    intro. inversion H.
-    exact (c_nat (S n)).
-    inversion P.
+  Instance carrier_eqdec A : EqDecision (carrier A).
+  Proof.
+    (* unfold EqDecision, Decision. *)
+    (* intros. *)
+    (* dependent induction x; dependent destruction y; auto. *)
+    (* destruct (decide (n = n0)) as [-> | ?]; [left; reflexivity | right; congruence]. *)
+    (* destruct (decide (b = b0)) as [-> | ?]; [left; reflexivity | right; congruence]. *)
+    (* destruct (IHx1 y1) as [-> | ?]; [| right; congruence]. *)
+    (* destruct (IHx2 y2) as [-> | ?]; [left; reflexivity | right; congruence]. *)
+    (* destruct (decide (A = A0)); [| right; congruence]. *)
+    (* destruct (IHx (eq_rect_r carrier y e)). *)
+    (* 2: { right. intro. inversion H. inversion_sigma. *)
+    (*   apply rew_swap in H2_0. rewrite (Eqdep.EqdepTheory.UIP _ _ _ H2_ e) in H2_0. *)
+    (*   apply n1. assumption. *)
+    (* } *)
+    (* pose proof (neqs_eq n (eq_rect_r (.≠ SortK) n0 e)). *)
+    (* left. Search eq_rect. *)
+  Admitted.
+
+  Definition DemoModel : @Model DemoSignature.
+  Proof.
+    unshelve eapply mkModel_singleton.
+    - exact carrier.
+    - destruct_with_eqn σ; simpl; intros.
+      * exact (c_nat 0).
+      * dependent induction H. exact (c_nat (S n)).
+        inversion P; subst. now apply IHcarrier.
+      * dependent induction H. dependent induction H0.
+        exact (c_nat (n + n0)).
+        inversion P; subst. now apply IHcarrier.
+        inversion P; subst. apply IHcarrier. reflexivity. exact H0. (* ? *)
+      * exact (c_bool true).
+      * exact (c_bool false).
+      * exact (c_bool false). (*TODO: I don't understand this still*)
+      * exact (c_nil).
+      * exact (c_cons H H0).
+      * dependent induction H0. exact (c_bool false).
+        dependent destruction H.
+        dependent destruction H0_.
+        destruct (decide (s0 = s1)). 2: exact (IHcarrier2 erefl).
+        destruct (decide (eq_rect_r carrier H e = H0_)).
+        exact (c_bool true). exact (IHcarrier2 erefl).
+        inversion P; subst. now apply IHcarrier.
+      * dependent induction H. exact H0. exact (IHcarrier2 erefl H0). (* ? *)
+        inversion P; subst. apply IHcarrier. reflexivity. exact H0. (* ? *)
+    - destruct s. 1-3,5: repeat constructor. do 2 econstructor; first last; repeat constructor. discriminate.
+    - intros. inversion H; subst. assumption. econstructor; eassumption.
   Defined.
-  Next Obligation.
-    simpl.
-    intros. inversion H. inversion H0.
-    exact (c_nat (n + n0)).
+
+  Definition test : @Theory DemoSignature.
+  Proof.
+    split. intros pat.
+    apply Logic.or.
+    refine (exists R, pat = existT R _).
+    eapply kore_equals. epose (kore_app SymTrue hnil). simpl in p. exact p.
+    epose (kore_app SymZero hnil). simpl in p.
+    epose (kore_inj _ _ p).
+    epose (kore_app SymSucc ⟨ p ⟩). simpl in p1. eapply kore_inj in p1.
+    epose (kore_app SymNil hnil). simpl in p2.
+    epose (kore_app SymCons ⟨ p0 ; p2 ⟩). simpl in p3.
+    epose (kore_app SymCons ⟨ p1 ; p3 ⟩). simpl in p4.
+    epose (kore_app SymInList ⟨ p0 ; p4 ⟩). simpl in p5.
+    exact p5. Unshelve. 1,3: right; discriminate.
+    apply Logic.or.
+    refine (exists R, pat = existT R _).
+    eapply kore_equals.
+    unshelve apply kore_app. exact SymAppend. simpl.
+    right. epose (kore_app SymNil hnil). simpl in p. exact p.
+    right. apply kore_fevar. exact "x".
+    left. simpl. apply kore_fevar. exact "x".
+    refine (exists R, pat = existT R _).
+    eapply kore_equals.
+    unshelve apply kore_app. exact SymAppend. simpl.
+    right. apply kore_fevar. exact "x".
+    right. epose (kore_app SymNil hnil). simpl in p. exact p.
+    left. simpl. apply kore_fevar. exact "x".
   Defined.
-  Next Obligation.
-    simpl.
-    exact (c_bool true).
-  Defined.
-  Next Obligation.
-    simpl.
-    exact (c_bool false).
-  Defined.
-  Next Obligation.
-    simpl.
-    Print DemoSyms.
-    intros.
-    inversion H. (* TODO *)
-  Defined.
-  Next Obligation.
-    simpl.
-    exact (c_nil).
-  Defined.
-  Next Obligation.
-    simpl.
-    intros.
-    exact (c_cons H H0).
-  Defined.
-  Next Obligation.
+
+  Goal satT test DemoModel.
+  Proof.
+    unfold satT, satM, test. intros.
+    inversion H; destruct H0; subst; simpl.
+    simplify_krule. give_up.
+    destruct H0; subst; simpl.
+    simplify_krule. reflexivity.
+    destruct H0; subst; simpl.
+    simplify_krule. unfold block, solution_left, eq_rec_r, eq_rect_r, carrier_rec. simpl. give_up.
+  Abort.
+
+  (* Program Definition DemoModel : @Model DemoSignature := *)
+  (*   mkModel_singleton *)
+  (*     carrier *)
+  (*     (DemoSyms_rect _ *)
+  (*       (c_nat 0) *)
+  (*       _ *)
+  (*       _ *)
+  (*       _ *)
+  (*       _ *)
+  (*       _ *)
+  (*       _ *)
+  (*       _ *)
+  (*       _ *)
+  (*     ) *)
+  (*     _ *)
+  (*     _. *)
+  (* Next Obligation. *)
+  (*   simpl. *)
+  (*   intro. inversion H. *)
+  (*   exact (c_nat (S n)). *)
+  (*   inversion P. *)
+  (* Defined. *)
+  (* Next Obligation. *)
+  (*   simpl. *)
+  (*   intros. inversion H. inversion H0. *)
+  (*   exact (c_nat (n + n0)). *)
+  (* Defined. *)
+  (* Next Obligation. *)
+  (*   simpl. *)
+  (*   exact (c_bool true). *)
+  (* Defined. *)
+  (* Next Obligation. *)
+  (*   simpl. *)
+  (*   exact (c_bool false). *)
+  (* Defined. *)
+  (* Next Obligation. *)
+  (*   simpl. *)
+  (*   Print DemoSyms. *)
+  (*   intros. *)
+  (*   inversion H. (1* TODO *1) *)
+  (* Defined. *)
+  (* Next Obligation. *)
+  (*   simpl. *)
+  (*   exact (c_nil). *)
+  (* Defined. *)
+  (* Next Obligation. *)
+  (*   simpl. *)
+  (*   intros. *)
+  (*   exact (c_cons H H0). *)
+  (* Defined. *)
+  (* Next Obligation. *)
 
